Generalize ELU to configurable alpha

dist/Kuiper_KB_Elu.h
@@ -5,13 +5,16 @@
 #include <kuiper.h>
 #include <kbench.h>
 
-void Kuiper_KB_Elu_elu_fw_f32(uint32_t lena, float *a);
+void Kuiper_KB_Elu_elu_fw_f32(float alpha, uint32_t lena, float *a);
 
-void Kuiper_KB_Elu_elu_fw_f64(uint32_t lena, double *a);
+void Kuiper_KB_Elu_elu_fw_f64(double alpha, uint32_t lena, double *a);
 
-float *Kuiper_KB_Elu_elu_alloc_f32(uint32_t lena, float *input);
+float *Kuiper_KB_Elu_elu_alloc_f32(float alpha, uint32_t lena, float *input);
 
-double *Kuiper_KB_Elu_elu_alloc_f64(uint32_t lena, double *input);
+double *Kuiper_KB_Elu_elu_alloc_f64(double alpha, uint32_t lena, double *input);
+
+float *Kuiper_KB_Elu_elu_alloc_f64_f32(double alpha, uint32_t lena,
+                                       float *input);
 
 #define Kuiper_KB_Elu_H_DEFINED
 #endif /* Kuiper_KB_Elu_H */
