src/kernelbench/level1/challenge31/Kuiper.KB.Elu.fst
@@ -4,26 +4,43 @@ module Kuiper.KB.Elu
 open Kuiper
 open Kuiper.Tensor
 open Kuiper.Kernel.Map
+open Kuiper.Float.Casts
 
 open Kuiper.Tensor.Layout.Alg { l1_forward }
 
-let elu_fw_f32 lena a #s = map_gpu elu_step lena a
-let elu_fw_f64 lena a #s = map_gpu elu_step lena a
+let elu_fw_f32 alpha lena a #s = map_gpu (elu_step alpha) lena a
+let elu_fw_f64 alpha lena a #s = map_gpu (elu_step alpha) lena a
 
 inline_for_extraction noextract
 fn elu_alloc (#t:Type0) {| floating t |}
+  (alpha : t)
   (lena : szp { lena <= max_blocks * max_threads })
   (input : array1 t (l1_forward lena) { is_global input })
   (#s : chest1 t lena) (#f : perm)
   norewrite
   preserves cpu ** on gpu_loc (input |-> Frac f s)
   returns output : array1 t (l1_forward lena)
-  ensures on gpu_loc (output |-> mk1 (fun i -> elu_step (acc1 s i)))
+  ensures on gpu_loc (output |-> mk1 (fun i -> elu_step alpha (acc1 s i)))
 {
   let output = alloc0 #t lena (l1_forward lena);
-  map_gpu_to elu_step lena input output;
+  map_gpu_to (elu_step alpha) lena input output;
   return output
 }
 
 let elu_alloc_f32 = elu_alloc #f32
 let elu_alloc_f64 = elu_alloc #f64
+
+fn elu_alloc_f64_f32
+  (alpha : f64)
+  (lena : szp { lena <= max_blocks * max_threads })
+  (input : array1 f32 (l1_forward lena) { is_global input })
+  (#s : chest1 f32 lena)
+  (#f : perm)
+  norewrite
+  preserves cpu ** on gpu_loc (input |-> Frac f s)
+  returns output : array1 f32 (l1_forward lena)
+  ensures on gpu_loc
+    (output |-> mk1 (fun i -> elu_step (fcast alpha) (acc1 s i)))
+{
+  elu_alloc #f32 (fcast alpha) lena input
+}
